spill_live: changed some definitions, fixed statement of the Lemma

theories/Spilling/Soundness.v
@@ -1,6 +1,6 @@
-Require Import List Map Env AllInRel Exp.
+Require Import List Map Env AllInRel Exp AppExpFree.
 Require Import IL Annotation InRel AutoIndTac Liveness LabelsDefined.
-Require Import SimI.
+Require Import SimI Spilling.
 
 Fixpoint write_spills (slot: var->var) (xs:list var) (s:stmt) : stmt :=
 match xs with
@@ -15,14 +15,397 @@ match xs with
 end.
 
 
-Fixpoint doSpill (slot: var -> var) (s:stmt) (a:ann (set var * set var)) : stmt :=
-match s, a with
-| stmtLet x e s, ann1 (Sp,L) a =>
-    write_spills slot (to_list Sp)
-                 (write_loads slot (to_list L) (stmtLet x e (doSpill slot s a)))
-| _,_ => s
+Fixpoint do_spill
+(slot: var -> var)
+(s:stmt)
+(sl:ann (set var * set var * option (list (set var * set var)))) : stmt :=
+
+let Sp := fst (fst (getAnn sl)) in
+let L  := snd (fst (getAnn sl)) in
+
+write_spills slot (elements Sp)
+  (write_loads slot (elements L)
+
+    (match s,sl with
+     | stmtLet x e s, ann1 _ sl_s
+       => stmtLet x e (do_spill slot s sl_s)
+     | stmtIf e s t, ann2 _ sl_s sl_t
+       => stmtIf e (do_spill slot s sl_s) (do_spill slot t sl_t)
+     | stmtFun F t, annF _ sl_F sl_t
+       => stmtFun
+            ((fun Zs sl_s => (fst Zs (* todo: really? I think it's fine *)
+                                    , do_spill slot (snd Zs) sl_s)) ⊜ F sl_F)
+            (do_spill slot t sl_t)
+
+     | _,_
+       => s
+     end))
+.
+
+Definition discard_sl := mapAnn (fun (a : (* = mapAnn ? snd *)
+      set var * set var * option (list (set var * set var)))
+                                           => match a with (_,_,rm) => rm end).
+
+Definition discard_merge_sl (slot : var -> var) :=
+mapAnn (fun (a : set var * set var * option (list (set var * set var)))
+         => match a with
+            | (_,_,None)
+              => None
+            | (_,_,Some rms)
+              => Some ((fun rm => match rm with
+                                  | (R,M) => R ∪ map slot M
+                                  end) ⊝ rms)
+            end).
+
+Fixpoint do_spill_rm
+(slot : var -> var)
+(sl: ann (set var * set var * option (list (set var * set var ))))
+: ann (set var * set var * option (list (set var * set var)))
+:=
+let add_nones := (fix f (n:nat)
+                        (b:ann(set var * set var * option(list(set var * set var))))
+                      := match n with
+                         |   0  => b
+                         | S(n) => ann1 (∅,∅,None) (f n b) end) in
+match sl with
+| ann0 (Sp,L,rm)           => add_nones (cardinal Sp + cardinal L)
+                                         sl
+| ann1 (Sp,L,rm) sl_s      => add_nones (cardinal Sp + cardinal L)
+                                        (ann1 (Sp,L,rm) (do_spill_rm slot sl_s))
+| ann2 (Sp,L,rm) sl_s sl_t => add_nones (cardinal Sp + cardinal L)
+                                        (ann2 (Sp,L,rm) (do_spill_rm slot sl_s)
+                                                        (do_spill_rm slot sl_t))
+| annF (Sp,L,rm) sl_F sl_t => add_nones (cardinal Sp + cardinal L)
+                                  (annF (Sp,L,rm) (do_spill_rm slot ⊝ sl_F)
+                                                  (do_spill_rm slot sl_t))
 end.
 
+
+Fixpoint spill_live
+(Lv : list (set var))
+(ZL : list (params))
+(G : set var)
+(s : stmt)
+(rm : ann (option (list (set var))))
+{struct s}
+: ann (set var)
+:=
+match s, rm with
+| stmtLet x e t, ann1 _ rm  (* checked *)
+     => let lv_t := spill_live Lv ZL (singleton x) t rm in
+        ann1 ((getAnn lv_t) \ singleton x ∪ Exp.freeVars e ∪ G) lv_t
+
+| stmtReturn e, ann0 _ (* checked *)
+     => ann0 (Op.freeVars e ∪ G)
+
+| stmtIf e t v, ann2 _ rm_t rm_v (* checked *)
+     => let lv_t := spill_live Lv ZL ∅ t rm_t in
+        let lv_v := spill_live Lv ZL ∅ v rm_v in
+        ann2 (getAnn lv_t ∪ getAnn lv_v ∪ Op.freeVars e ∪ G) lv_t lv_v
+
+| stmtApp f Y, ann0 _ (* checked *)
+     => let blv := nth (counted f) Lv ∅ in
+        let Z   := nth (counted f) ZL nil in
+        (* attention: (forall (n : nat) (y : op), get Y n y -> live_op_sound y lv) *)
+        ann0 (blv \ of_list Z ∪ G)
+
+| stmtFun F t, annF (Some Lv') rm_F rm_t (* checked *)
+     => let lv_t := spill_live (Lv' ++ Lv) (fst ⊝ F ++ ZL) ∅ t rm_t in
+        let lv_F := (fun ps rm_s
+                 => spill_live (Lv' ++ Lv) (fst ⊝ F ++ ZL) ∅
+                               (snd ps) rm_s) ⊜ F rm_F in
+        (* maybe i will need a guarantee of ❬F❭ = ❬als❭ somewhere *)
+        annF (getAnn lv_t ∪ G) lv_F lv_t
+
+| _,_ => ann0 ∅
+
+end.
+
+Lemma write_spills_empty
+(slot : var -> var)
+(s : stmt)
+: write_spills slot nil s = s.
+Proof.
+simpl.
+eauto.
+Qed.
+
+Lemma write_loads_empty
+(slot : var -> var)
+(s : stmt)
+: write_loads slot nil s = s.
+Proof.
+simpl.
+eauto.
+Qed.
+(*
+Lemma do_spill_empty_let
+(slot : var -> var)
+(Λ : list (set var * set var))
+(ZL : list params)
+(Lv : list (set var))
+(x : var)
+(e : exp)
+(s : stmt)
+(sl : ann (set var * set var * option (list (set var * set var))))
+:    live_sound Imperative ZL Lv
+          (do_spill slot (stmtLet x e s) (ann1 (∅,∅,None) sl))
+     (spill_live slot Λ ZL
+          (do_spill slot (stmtLet x e s) (ann1 (∅,∅,None) sl))
+          (ann1 None (discard_sl sl)))
+
+  -> live_sound Imperative ZL Lv
+          (stmtLet x e (do_spill slot s sl))
+     (spill_live slot Λ ZL
+          (stmtLet x e (do_spill slot s sl))
+          (ann1 None (discard_sl sl))).
+Proof.
+intros lvSound.
+simpl.
+inversion_clear lvSound.
+rewrite elements_empty in H.
+rewrite write_loads_empty in H.
+rewrite write_spills_empty in H.
+
+rewrite elements_empty in H0.
+rewrite write_loads_empty in H0.
+rewrite write_spills_empty in H0.
+
+rewrite elements_empty in H1.
+rewrite write_loads_empty in H1.
+rewrite write_spills_empty in H1.
+
+rewrite elements_empty in H2.
+rewrite write_loads_empty in H2.
+rewrite write_spills_empty in H2.
+
+simpl in *.
+
+econstructor; simpl; eauto.
+Qed.
+
+Lemma do_spill_empty_let'
+(slot : var -> var)
+(Λ : list (set var * set var))
+(ZL : list params)
+(Lv : list (set var))
+(x : var)
+(e : exp)
+(s : stmt)
+(lv : ann (set var))
+(sl : ann (set var * set var * option (list (set var * set var))))
+:    live_sound Imperative ZL Lv
+          (do_spill slot (stmtLet x e s) (ann1 (∅,∅,None) sl))
+          lv
+
+  -> live_sound Imperative ZL Lv
+          (stmtLet x e (do_spill slot s sl))
+          lv.
+Proof.
+intros lvSound.
+simpl.
+inversion_clear lvSound.
+rewrite elements_empty in H.
+rewrite write_loads_empty in H.
+rewrite write_spills_empty in H.
+
+rewrite elements_empty in H0.
+rewrite write_loads_empty in H0.
+rewrite write_spills_empty in H0.
+
+rewrite elements_empty in H1.
+rewrite write_loads_empty in H1.
+rewrite write_spills_empty in H1.
+
+rewrite elements_empty in H2.
+rewrite write_loads_empty in H2.
+rewrite write_spills_empty in H2.
+
+simpl in *.
+
+econstructor; simpl; eauto.
+Qed.
+
+Lemma do_spill_empty_if
+(slot : var -> var)
+(Λ : list (set var * set var))
+(ZL : list params)
+(Lv : list (set var))
+(lv : ann (set var))
+(e : op)
+(s t : stmt)
+(sl_s sl_t : ann (set var * set var * option (list (set var * set var))))
+:    live_sound Imperative ZL Lv
+          (do_spill slot (stmtIf e s t) (ann2 (∅,∅,None) sl_s sl_t))
+          lv
+
+  -> live_sound Imperative ZL Lv
+          (stmtIf e (do_spill slot s sl_s) (do_spill slot t sl_t))
+          lv.
+Proof.
+intros lvSound.
+simpl.
+inversion_clear lvSound.
+
+rewrite elements_empty in H.
+rewrite write_loads_empty in H.
+rewrite write_spills_empty in H.
+
+rewrite elements_empty in H0.
+rewrite write_loads_empty in H0.
+rewrite write_spills_empty in H0.
+
+rewrite elements_empty in H1.
+rewrite write_loads_empty in H1.
+rewrite write_spills_empty in H1.
+
+simpl in *.
+
+econstructor; simpl; eauto.
+Qed.
+*)
+(*
+Lemma do_spill_empty
+(slot : var -> var)
+(Λ : list (set var * set var))
+(ZL : list params)
+(Lv : list (set var))
+(s : stmt)
+(sl : ann (set var * set var * option (list (set var * set var))))
+: live_sound Imperative ZL Lv (do_spill slot s sl)
+        (spill_live slot Λ ZL (do_spill slot s sl) sl)
+    -> fst (getAnn sl) === (∅,∅) ->
+ match s, sl with
+  | stmtLet x e t, ann1 (_,_,_) sl_t
+    => live_sound Imperative ZL Lv (stmtLet x e (do_spill slot t sl_t))
+             (spill_live slot Λ ZL (stmtLet x e (do_spill slot t sl_t)) sl)
+  | stmtIf e t v, ann2 (_,_,_) sl_t sl_v
+    => live_sound Imperative ZL Lv (stmtIf e (do_spill slot t sl_t)
+                                             (do_spill slot v sl_v))
+             (spill_live slot Λ ZL (stmtIf e (do_spill slot t sl_t)
+                                             (do_spill slot v sl_v)) sl)
+  | _,_ => True
+end.
+Proof.
+intros lvSound fstEmpty.
+destruct s,sl ; simpl; eauto.
+- intros.
+
+
+apply IHlvSound; simpl.
+- admit.
+- admit.
+Admitted.
+
+*)
+
+Definition slot_merge slot := List.map (fun (RM : set var * set var)
+                                           => fst RM ∪ map slot (snd RM)).
+
+Lemma spill_live_sound
+(k : nat)
+(slot : var -> var) (*maybe needs restrictions*)
+(ZL : list params)
+(G : set var)
+(Λ : list (set var * set var))
+(R M : set var)
+(Lv : list (set var))
+(s : stmt)
+(sl : ann (set var * set var * option (list (set var * set var))))
+(alv : ann (set var))
+:  app_expfree s
+-> spill_sound k ZL Λ (R,M) s sl
+-> live_sound Imperative ZL Lv s alv
+-> live_sound Imperative ZL Lv
+              (do_spill slot s sl)
+              (spill_live (slot_merge slot Λ) ZL G
+                          (do_spill slot s sl)
+                          (discard_merge_sl slot (do_spill_rm slot sl))).
+
+Proof.
+intros aeFree spillSound lvSound.
+(*induction (elements (fst (fst (getAnn sl)))).
+general induction spillSound; inversion_clear lvSound; inversion_clear aeFree;
+simpl.
+*)
+
+general induction lvSound; inversion_clear spillSound;
+
+inversion_clear aeFree as [x' e' s' eaFree_s
+                          |e'
+                          |e' s' t' aeFree_s eaFree_t
+                          |f' Y' aeFree_var
+                          |F' t' aeFree_F aeFree_t]. simpl; eauto.
+(*
+induction (elements Sp); induction (elements L).
+- admit.
+- admit.
+- admit.
+-
+try rewrite write_loads_empty; try rewrite write_spills_empty; simpl; eauto;*)
+
+- (*revert dependent sl.*) induction (elements Sp); induction (elements L).
+  (*intros sl0 H7.*)
+  + rewrite write_spills_empty. rewrite write_loads_empty.
+    simpl. econstructor.
+    * eapply IHspillSound; eauto.
+    * apply live_exp_sound_incl with (lv':=Exp.freeVars e).
+      -- apply Exp.live_freeVars.
+      -- cset_tac.
+    * eauto.
+    * admit.
+  + rewrite write_spills_empty.
+    rewrite write_spills_empty in IHl.
+    simpl. econstructor.
+    * admit.
+    * econstructor. econstructor. cset_tac.
+    * eauto.
+    * revert a. admit. (*this is unprovable*)
+  + rewrite write_loads_empty.
+    rewrite write_loads_empty in IHl.
+    simpl. econstructor.
+    * admit.
+    * econstructor. econstructor. cset_tac.
+    * eauto.
+    * admit. (*this is unprovable*)
+  + admit.
+- induction (elements Sp); induction (elements L).
+  + rewrite write_loads_empty. rewrite write_spills_empty.
+    simpl. econstructor. apply Op.live_freeVars.
+  + rewrite write_spills_empty.
+    rewrite write_spills_empty in IHl.
+    simpl. eapply LOpr.
+
+- apply live_exp_sound_incl with (lv':=Exp.freeVars e).
+  + apply Exp.live_freeVars.
+  + cset_tac.
+- admit.
+- admit.
+- econstructor. econstructor. cset_tac.
+- simpl. induction (elements Sp), (elements L); simpl.
+  + econstructor; eauto.
+    * apply live_exp_sound_incl with (lv':=Exp.freeVars e).
+      -- apply Exp.live_freeVars.
+      -- cset_tac.
+    * admit. (*Why do we need this condition?*)
+  + admit.
+  + admit.
+  + admit.
+- apply do_spill_empty_if in IHlvSound1.
+  apply do_spill_empty_if.
+  +
+enough (forall sl1 sl2, live_sound Imperative ZL Lv (do_spill slot s1
+   (ann2 (∅,∅,None) sl1 sl2))
+   (spill_live slot Λ ZL (do_spill slot s1 (ann2 (∅,∅,None) sl1 sl2))
+                                           (ann2 (∅,∅,None) sl1 sl2))
+  -> live_sound Imperative ZL Lv (stmtIf e ).
+   * apply H8.
+eapply IHlvSound1. ; admit.
+- econstructor; admit.
+- econstructor. apply Op.live_freeVars.
+- econstructor; admit.
+
+Op.live_freeVars
 
 Theorem spill_sound_correct L E E' : spill_sound k Lsl (R,M) s alv asl
 -> (forall x : var, In x R -> E x = E' x)
